proofs/fstar/extraction-edited/Libcrux.Kem.Kyber.fsti
@@ -3,17 +3,6 @@ module Libcrux.Kem.Kyber
 open Core
 open FStar.Mul
 
-val serialize_kem_secret_key (#p:Spec.Kyber.params)
-      (v_SERIALIZED_KEY_LEN: usize)
-      (private_key public_key implicit_rejection_value: t_Slice u8)
-    : Pure (t_Array u8 v_SERIALIZED_KEY_LEN)
-      (requires (length private_key == Spec.Kyber.v_CPA_PKE_SECRET_KEY_SIZE p /\
-                 length public_key == Spec.Kyber.v_CPA_PKE_PUBLIC_KEY_SIZE p /\
-                 length implicit_rejection_value == Spec.Kyber.v_SHARED_SECRET_SIZE /\
-                 v_SERIALIZED_KEY_LEN == Spec.Kyber.v_SECRET_KEY_SIZE p))
-      (ensures (fun res -> res == Spec.Kyber.ind_cpa_serialize_secret_key p (private_key,public_key) implicit_rejection_value))
-                 
-
 val decapsulate (#p:Spec.Kyber.params)
       (v_K v_SECRET_KEY_SIZE v_CPA_SECRET_KEY_SIZE v_PUBLIC_KEY_SIZE v_CIPHERTEXT_SIZE v_T_AS_NTT_ENCODED_SIZE v_C1_SIZE v_C2_SIZE v_VECTOR_U_COMPRESSION_FACTOR v_VECTOR_V_COMPRESSION_FACTOR v_C1_BLOCK_SIZE v_ETA1 v_ETA1_RANDOMNESS_SIZE v_ETA2 v_ETA2_RANDOMNESS_SIZE v_IMPLICIT_REJECTION_HASH_INPUT_SIZE:
           usize)
